Added inductive definition for CPS translation.
Shows only the show cases.

Coq Developments/msci/CPS_Translation.v
@@ -1,6 +1,6 @@
 (** Beginning of the file defining the translation from GV to CP. *)
 Require Import Metatheory.
-Require Import CP_Definitions CP_Typing GV_Definitions.
+Require Import CP_Definitions CP_Typing GV_Definitions GV_Infrastructure.
 Require Import ExtLib.Structures.Applicative.
 Require Import ExtLib.Structures.Functor.
 Require Import ExtLib.Structures.Monad.
@@ -25,15 +25,15 @@ Fixpoint trans_types (T:typ) : prop :=
     | typ_iend => pp_one
     | A <x> B => ⟦A⟧t ⨂ ⟦B⟧t
     | A ⊸ B => (¬⟦A⟧t) ⅋ ⟦B⟧t
-    | A → B => pp_accept ((¬⟦A⟧t) ⅋ ⟦B⟧t)
+    | A ⟶ B => pp_accept ((¬⟦A⟧t) ⅋ ⟦B⟧t)
     | typ_unit => pp_accept pp_top
   end
 where "'⟦' T '⟧t'" := (trans_types T).
 
 Fixpoint infer (tm:term) (G:tenv) (xs:list typ) : option typ :=
   let flip t := match t with
-                   | T ⊸ U => T → U
-                   | T → U => T ⊸ U
+                   | T ⊸ U => T ⟶ U
+                   | T ⟶ U => T ⊸ U
                    | _ => t
                 end
   in
@@ -75,10 +75,73 @@ Fixpoint infer (tm:term) (G:tenv) (xs:list typ) : option typ :=
     | tm_end _ => Some typ_unit
   end.
 
+Inductive inferTy : term -> tenv -> typ -> Prop :=
+  | infer_fvar: forall x G T (RET: get x G = Some T),
+                  inferTy (tm_var (fvar x)) G T
+  | infer_unit: forall G, inferTy tm_unit G typ_unit
+  | infer_weak: forall (x:atom) M G T U (INF: inferTy M G T),
+                  inferTy (tm_weak x M) (x ~ U ++ G) T
+  | infer_abs: forall L M G T U
+                      (INF: forall x (NIN: x `notin` L),
+                              inferTy (open M x) (x~T ++ G) U),
+                 inferTy (tm_abs T M) G (T ⊸ U)
+  | infer_iabs: forall M G T U (INF: inferTy M G (T ⊸ U)),
+                  inferTy (tm_iabs M) G (T ⟶ U)
+  | infer_eabs: forall M G T U (INF: inferTy M G (T ⟶ U)),
+                  inferTy (tm_eabs M) G (T ⊸ U)
+  | infer_app: forall M N G H T U
+                      (INFM: inferTy M G (T ⊸ U))
+                      (INFN: inferTy N H T),
+                 inferTy (tm_app M N) (G++H) U
+  | infer_pair: forall M N G H T U
+                      (INFM: inferTy M G T)
+                      (INFN: inferTy N H U),
+                  inferTy (tm_pair M N) (G++H) (T <x> U)
+  | infer_let:
+      forall L M N G H T U V
+             (INFM: inferTy M G (T <x> U))
+             (INFN: forall x y
+                           (NINX: x `notin` L)
+                           (NINY: y `notin` L `union` singleton x),
+                      inferTy ({1 ~> x}(open N y)) (x ~ T ++ y ~ U ++ H) V),
+        inferTy (tm_let T U M N) (G++H) V
+  | infer_send: forall M N G H T U
+                       (INFM: inferTy M G T)
+                       (INFN: inferTy N H (! T # U)),
+                  inferTy (tm_send M N) (G++H) U
+  | infer_recv: forall M G T U
+                       (INFM: inferTy M G (? T # U)),
+                  inferTy (tm_recv M) G (T <x> U)
+  | infer_select_inl: forall M G S1 S2
+                             (INFM: inferTy M G (S1 <+> S2)),
+                    inferTy (tm_select lb_inl M) G S1
+  | infer_select_inr: forall M G S1 S2
+                             (INFM: inferTy M G (S1 <+> S2)),
+                        inferTy (tm_select lb_inr M) G S2
+  | infer_case: forall L M NL NR G H S1 S2 T
+                       (INFM: inferTy M G (S1 <&> S2))
+                       (INFNL: forall x (NIN: x `notin` L),
+                                 inferTy (open NL x) (x ~ S1 ++ H) T)
+                       (INFNR: forall x (NIN: x `notin` L),
+                                 inferTy (open NR x) (x ~ S2 ++ H) T),
+                  inferTy (tm_case M NL NR) (G++H) T
+  | infer_connect: forall L M N G H T dT U
+                          (DUA: are_dual T dT)
+                          (INFM: forall x (NIN: x `notin` L),
+                                   inferTy (open M x) (x ~ T ++ G) typ_oend)
+                          (INFN: forall x (NIN: x `notin` L),
+                                   inferTy (open N x) (x ~ dT ++ H) U),
+                     inferTy (tm_connect T M N) (G++H) U
+  | infer_end: forall M G (INF: inferTy M G typ_iend),
+                 inferTy (tm_end M) G typ_unit.
+
+Hint Constructors inferTy.
+
 Lemma somm:
-  forall Φ M T (WT: Φ ⊢ M ∈ T), infer M Φ nil = Some T.
+  forall Φ M T (WT: Φ ⊢ M ∈ T), inferTy M Φ T.
 Proof.
-Admitted.
+  ii; induction WT; try (solve [eauto|constructor; ss; des; tryfalse; eauto]).
+Qed.
 
 Fixpoint trans_tm' (tm:term) (G:tenv) (xs:list typ) (z:pname) : option proc :=
   match tm with
@@ -160,6 +223,88 @@ Fixpoint trans_tm' (tm:term) (G:tenv) (xs:list typ) (z:pname) : option proc :=
          ret $ p_par pp_one M' (p_empin 0 (p_accept z pp_top (0 CASE 0)))
   end.
 
+Inductive transTm : term -> tenv -> pname -> proc -> Prop :=
+  | trans_fvar: forall x G z,
+                  transTm (tm_var (fvar x)) G z (x ⟷ z)
+  | trans_unit: forall G z,
+                  transTm tm_unit G z (! ⟨pp_top⟩z → (0 CASE 0))
+  | trans_weak: forall (x:atom) T M P G z
+                       (TR: transTm M G z P),
+                  transTm (tm_weak x M) (x ~ T ++ G) z (? []x → P)
+  | trans_abs: forall L T M P G z
+                      (TR: forall x (NIN: x `notin` L),
+                             transTm (open M x) (x ~ T ++ G) z P),
+                 transTm (tm_abs T M) G z (⟨¬⟦T⟧t⟩z → P)
+  | trans_iabs: forall T M P G z
+                       (INF: inferTy M G T)
+                       (TR: transTm M G 0 P),
+                  transTm (tm_iabs M) G z (! ⟨⟦T⟧t⟩z → P)
+  | trans_eabs:
+      forall T M P G z
+             (INF: inferTy M G T)
+             (TR: transTm M G 0 P),
+        transTm (tm_eabs M) G z
+                (ν (pp_accept (⟦T⟧t)) → P ‖ ? [¬⟦T⟧t]0 → (0 ⟷ z))
+  | trans_app:
+      forall T U M N P Q G H z
+             (INFM: inferTy M G T)  (INFN: inferTy N H U)
+             (TRM: transTm M G 0 P) (TRN: transTm N H 0 Q),
+        transTm (tm_app M N) (G++H) z (ν ⟦T⟧t → P ‖ [⟦T⟧t]0 → Q ‖ 1 ⟷ z)
+  | trans_pair:
+      forall T M N P Q G H z
+             (INFM: inferTy M G T)
+             (TRM: transTm M G 0 P) (TRN: transTm N H 0 Q),
+        transTm (tm_pair M N) (G++H) z ([⟦T⟧t]z → P ‖ Q)
+  | trans_let:
+      forall L T U M N P Q G H z
+             (TR: transTm M G 0 P)
+             (TRN: forall x y
+                          (NINX: x `notin` L)
+                          (NINY: y `notin` L `union` singleton x),
+                     transTm ({1 ~> x}(open N y)) H z Q),
+        transTm (tm_let T U M N) (G++H) z
+                (ν ⟦T <x> U⟧t → P ‖ ⟨¬⟦T⟧t⟩0 → Q)
+  | trans_send:
+      forall T U M N P Q G H z
+             (INFM: inferTy M G T)  (INFN: inferTy N H U)
+             (TRM: transTm M G 0 P) (TRN: transTm M H 0 Q),
+        transTm (tm_send M N) (G++H) z
+                (ν ⟦U⟧t → ([⟦T⟧t]0 → P ‖ 0 ⟷ z) ‖ Q)
+  | trans_recv:
+      forall M P G z (TR: transTm M G z P),
+        transTm (tm_recv M) G z P
+  | trans_select_inl:
+      forall T M P G z
+             (INF: inferTy M G T)
+             (TR: transTm M G 0 P),
+        transTm (tm_select lb_inl M) G z (ν ⟦T⟧t → P ‖ 0[inl] → 0 ⟷ z)
+  | trans_select_inr:
+      forall T M P G z
+             (INF: inferTy M G T)
+             (TR: transTm M G 0 P),
+        transTm (tm_select lb_inr M) G z (ν ⟦T⟧t → P ‖ 0[inr] → 0 ⟷ z)
+  | trans_case:
+      forall L S1 S2 M NL NR P QL QR G H z
+             (INFM: inferTy M G (S1 <&> S2))
+             (TRNL: forall x (NIN: x `notin` L),
+                       transTm (open NL x) (x ~ S1 ++ H) z QL)
+             (TRNR: forall x (NIN: x `notin` L),
+                       transTm (open NR x) (x ~ S2 ++ H) z QR),
+        transTm (tm_case M NL NR) (G++H) z
+                (ν ⟦S1 <&> S2⟧t → P ‖ 0 CASE QL OR QR)
+  | trans_connect:
+      forall L T dT M N P Q G H z
+             (DUA: are_dual T dT)
+             (TRM: forall x (NIN: x `notin` L),
+                     transTm (open M x) (x ~ T ++ G) 0 P)
+             (TRN: forall x (NIN: x `notin` L),
+                     transTm (open N x) (x ~ dT ++ H) z Q),
+        transTm (tm_connect T M N) (G++H) z
+                (ν ¬⟦T⟧t → (ν pp_bot → P ‖ 0 → 0) ‖ Q)
+  | trans_end:
+      forall M P G z (TR: transTm M G 0 P),
+        transTm (tm_end M) G z (ν pp_one → P ‖ ⟨⟩0 → ⟨pp_top⟩z → (0 CASE 0)).
+
 (** Translation of terms. *)
 Definition trans_tm M G z := trans_tm' M G nil z.
 
@@ -188,5 +333,6 @@ Proof.
     simpl_env.
     pick fresh y and apply cp_accept; eauto.
     rewrite /open_proc; s; simpl_env; eauto.
+  - admit.
   -
 Admitted.
